src/basicmodal/semantics/consistency.lean
@@ -2,8 +2,8 @@
 -- Hans van Ditmarsch, Wiebe van der Hoek, and Barteld Kooi
 
 import basicmodal.language basicmodal.syntax.syntax 
-import basicmodal.semantics.semantics 
-import basicmodal.syntax.syntaxlemmas order.zorn data.set.basic
+import basicmodal.semantics.semantics basicmodal.syntax.syntaxlemmas
+import basicmodal.syntax.soundness order.zorn data.set.basic
 local attribute [instance] classical.prop_decidable
 
 open prfK
@@ -19,10 +19,11 @@ def fin_conj : list form → form
 
 
 -- a few helper lemmas about finite conjunctions
-lemma fin_conj_simp : ∀ Γ, ∀ ψ : form, prfK Γ (¬fin_conj [ψ, ¬ψ]) :=
+lemma fin_conj_simp {Γ : ctx} : ∀ ψ : form, prfK Γ (¬fin_conj [ψ, ¬ψ]) :=
 begin
-intros Γ ψ, simp, rw fin_conj, rw fin_conj, rw fin_conj, simp,
-have h2 : (prfK Γ (((¬ψ)&⊤) ↔ (¬ψ)) → (prfK Γ (¬(ψ & ((¬ψ)&⊤))) ↔ prfK Γ (¬(ψ & (¬ψ))))), 
+intro ψ, simp, rw fin_conj, rw fin_conj, rw fin_conj, simp,
+have h2 : (prfK Γ (((¬ψ)&⊤) ↔ (¬ψ)) → 
+  (prfK Γ (¬(ψ & ((¬ψ)&⊤))) ↔ prfK Γ (¬(ψ & (¬ψ))))), 
   from not_and_subst,
 simp at h2,
 specialize h2 phi_and_true, cases h2,
@@ -53,14 +54,53 @@ exact mp (mp pl4 (cut (mp pl5 and_commute) (imp_and_imp (mp pl5 L'_ih))))
   (cut iden (cut (imp_and_imp (mp pl6 L'_ih)) (mp pl6 and_commute)))
 end 
 
+lemma nprfalse : ¬ prfK ∅ ⊥ :=
+begin
+have h1 : ¬ sem_csq ∅ ⊥ → ¬ prfK ∅ ⊥, from soundness2 ∅ ⊥,
+apply h1,
+by_contradiction h2,
+rw sem_csq at h2,
+let f : frame := { states := nat,
+  h := ⟨0⟩,
+  rel := λ x y : nat, x = y }, 
+specialize h2 f,
+let v : nat → f.states → Prop := λ n x, true,
+specialize h2 v,
+let x : f.states := 42,
+specialize h2 x,
+apply h2,
+intros y φ h3,
+have h4 : φ ∉ ∅, {exact list.not_mem_nil φ},
+exact absurd h3 h4
+end
 
+
+lemma fin_conj_empty {AX : ctx} {L : list form} :
+  L = [] → ¬ prfK AX (fin_conj L ⊃ ⊥) :=
+begin
+intro h1, subst h1, rw fin_conj, simp at *,
+have h1 : prfK AX (¬⊥), from iden,
+simp at *, by_contradiction h2,
+have h3 : prfK AX ⊥, from mp h2 h1,
+have h4 : ¬ prfK AX ⊥, sorry,
+exact absurd h3 h4
+end 
 
 -- consistency for a finite set of formulas L
 def fin_ax_consist (AX : ctx) (L : list form) := ¬ prfK AX (fin_conj L ⊃ ⊥)
 
+
 -- consistency for an arbitrary set of formulas Γ
 def ax_consist (AX Γ : ctx) := 
   ∀ L : list form, (∀ ψ ∈ L, ψ ∈ Γ) → fin_ax_consist AX L
+ 
+-- -- consistency for an arbitrary set of formulas Γ
+-- def ax_consist' (AX : ctx) : ctx → list form → Prop
+-- | Γ [] := fin_ax_consist AX []
+-- | Γ L := (∀ ψ ∈ L, ψ ∈ Γ) → fin_ax_consist AX L
+
+-- #check ax_consist'
+
 
 -- Γ is maximally ax-consistent
 def max_ax_consist (AX Γ : ctx) := 
@@ -77,21 +117,24 @@ lemma five_helper (AX : ctx) :
   (∀ ψ ∈ L, ψ ∈ Γ ∨ ψ = φ) → prfK AX (fin_conj L ⊃ b) → ∃ L',
   (∀ ψ ∈ L', ψ ∈ Γ) ∧ prfK AX (fin_conj L' ⊃ (φ ⊃ b)) :=
 begin
-intros Γ φ L b h1 h2, revert b, induction L,
-{intros b h2, existsi ([] : list form), split, intros ψ h3, exfalso, 
-apply list.not_mem_nil ψ h3, dsimp [fin_conj] at *,
-have h3 := imp_if_imp_imp h2, exact h3},
-{have h1a : ∀ (ψ : form), ψ ∈ L_tl → ψ ∈ Γ ∨ ψ = φ, 
-{intros ψ h2, specialize h1 ψ, 
-have h3 := list.subset_cons L_hd L_tl,
-have h4 := list.mem_cons_of_mem L_hd h2, 
-apply h1 h4},
-intros b h2, 
+intros Γ φ L b h1 h2, 
+revert b, 
+induction L,
+{intros b h2, existsi ([] : list form), split, 
+intros ψ h3, exfalso, apply list.not_mem_nil ψ h3, 
+dsimp [fin_conj] at *, exact imp_if_imp_imp h2},
+{intros b h2,
+have h1a : ∀ (ψ : form), ψ ∈ L_tl → ψ ∈ Γ ∨ ψ = φ, 
+  {intros ψ h2, specialize h1 ψ, 
+  have h3 := list.subset_cons L_hd L_tl,
+  have h4 := list.mem_cons_of_mem L_hd h2, 
+  apply h1 h4},
+specialize L_ih h1a,
 have h1b: L_hd ∈ Γ ∨ L_hd = φ, 
-{apply h1 L_hd, left, refl},
-specialize L_ih h1a, cases h1b, 
-{have h3 : prfK AX (fin_conj L_tl ⊃(L_hd ⊃ b)),
-rw imp_conj_imp_imp at h2, exact h2, exact b,
+  {apply h1 L_hd, left, refl},
+cases h1b, 
+have h3 : prfK AX (fin_conj L_tl ⊃ (L_hd ⊃ b)), 
+  from and_right_imp.mp h2,
 specialize L_ih (L_hd ⊃ b) h3,
 cases L_ih with L' ih, existsi (L_hd::L' : list form),
 cases ih, split, intros ψ h4, cases h4, 
@@ -99,10 +142,17 @@ subst h4, exact h1b,
 apply ih_left ψ h4, rw imp_shift at ih_right,
 rw ←imp_conj_imp_imp at ih_right, exact ih_right,
 have h3 : prfK AX (fin_conj (L_hd::L_tl) ⊃ b), 
-exact h2, exact b},
-{have h4 : prfK AX (fin_conj L_tl ⊃ b), {sorry},
-specialize L_ih b h4, cases L_ih with L' ih, 
-existsi (L' : list form), exact ih}}
+exact h2, exact b,
+specialize L_ih (φ ⊃ b),
+have h5 : prfK AX (fin_conj (L_hd :: L_tl) ⊃ b) → 
+  prfK AX (fin_conj L_tl ⊃ (L_hd ⊃ b)), 
+  from and_right_imp.mp,
+specialize h5 h2,
+have h6 : prfK AX (fin_conj L_tl ⊃ (φ ⊃ b)), 
+  from eq.subst h1b h5,
+specialize L_ih h6, cases L_ih with L' ih, 
+cases ih, existsi (L' : list form), split, 
+exact ih_left, exact imp_imp_iff_imp.mp ih_right}
 end
 
 
@@ -111,15 +161,16 @@ lemma five (AX : ctx) :
   ∀ Γ : ctx, ∀ φ : form, ¬ ax_consist AX (Γ ∪ φ) → ∃ L',
   (∀ ψ ∈ L', ψ ∈ Γ) ∧ prfK AX (fin_conj L' ⊃ ¬φ) :=
 begin
-intros Γ φ h1, simp at *, rw ax_consist at h1, rw not_forall at h1,
-cases h1 with L h1, rw not_imp at h1, cases h1, 
-rw fin_ax_consist at h1_right, rw not_not at h1_right,
-existsi (L : list form), split,
-intros ψ h, 
-specialize h1_left ψ h,
-sorry, sorry 
+intro Γ, intro φ, intro h1, simp at *, rw ax_consist at h1, rw not_forall at h1,
+cases h1 with L h1, rw not_imp at h1,
+have h2 : (∀ ψ ∈ L, ψ ∈ Γ ∨ ψ = φ) → prfK AX (fin_conj L ⊃ ⊥) → ∃ L',
+  (∀ ψ ∈ L', ψ ∈ Γ) ∧ prfK AX (fin_conj L' ⊃ (φ ⊃ ⊥)), from five_helper AX Γ φ L ⊥,
+cases h1,
+have h3 : (∀ (ψ : form), ψ ∈ L → ψ ∈ Γ ∨ ψ = φ), 
+{intros ψ this, specialize h1_left ψ this, exact or.swap h1_left},
+specialize h2 h3, apply h2, rw fin_ax_consist at h1_right, rw not_not at h1_right,
+exact h1_right,
 end
-
 
 -- lemma 6 from class notes
 lemma six (AX Γ Γ' : ctx) (h : ax_consist AX Γ) :
@@ -131,14 +182,14 @@ cases h2 with h2l h2r, rw max_ax_consist at h1,
 cases h1 with h1l h1r, clear h, 
 have h2 := h1r (Γ ∪ φ), simp at h2, have h3 := h1r (Γ ∪ ¬φ),
 simp at h3, have h4 : ¬ax_consist AX (Γ ∪ ¬φ), 
-{simp at *, apply h3, rw set.ssubset_def, 
+{simp at *, apply h3, rw set.ssubset_iff_subset_not_subset, 
 split, 
 rw set.subset_def, intros x h4, exact or.inr h4,
 rw set.not_subset, existsi (¬φ : form), simp, split, 
 apply set.mem_union_left, rw set.mem_def, exact h2r},
 have h5 : ¬ax_consist AX (Γ ∪ φ), 
 {simp at *, apply h2,
-rw set.ssubset_def, 
+rw set.ssubset_iff_subset_not_subset, 
 split, 
 rw set.subset_def, intros x h4, exact or.inr h4,
 rw set.not_subset, existsi (φ : form), split, 
@@ -160,7 +211,7 @@ specialize h1l h13, exact absurd h12 h1l,
 exact h4,
 exact h5},
 {intro h1, dsimp at h1, rw max_ax_consist, split, exact h,
-intro Γ', intro h2, rw set.ssubset_def at h2, cases h2,
+intro Γ', intro h2, rw set.ssubset_iff_subset_not_subset at h2, cases h2,
 rw set.not_subset at h2_right,
 apply (exists.elim h2_right), simp, intros ψ h3 h4,
 specialize h1 ψ, cases h1, apply absurd h1 h4,
@@ -168,7 +219,7 @@ have h5 : (¬ψ) ∈ Γ', from set.mem_of_subset_of_mem h2_left h1,
 rw ax_consist, rw not_forall, existsi ([ψ,¬ψ] : list form),
 simp, split, intros φ h6, cases h6, subst h6, exact h3, 
 subst h6, exact h5, rw fin_ax_consist, rw not_not,
-exact fin_conj_simp AX ψ}
+exact fin_conj_simp ψ}
 end
 
 
@@ -181,14 +232,16 @@ split,
 {intro h1, split, rw max_ax_consist at h1, exact h1.left, 
 intros Γ' h2 h3, rw set.subset.antisymm_iff, split, exact h3,
 by_contradiction h4, rw max_ax_consist at h1, cases h1, 
-have h5 := and.intro h3 h4, rw ←set.ssubset_def at h5,
-specialize h1_right Γ' h5, exact h1_right h2}, 
+have h5 := and.intro h3 h4, 
+have h6 : Γ ⊂ Γ', from set.ssubset_iff_subset_not_subset.mpr h5,
+specialize h1_right Γ' h6, exact h1_right h2}, 
 intro h1, cases h1, rw max_ax_consist, split, exact h1_left,
 intros Γ' h2, by_contradiction h3, specialize h1_right Γ' h3,
 rw set.ssubset_def at h2, cases h2, apply h2_right, rw h1_right h2_left
 end
 
 open zorn
+
 lemma lindenbaum (AX Γ : ctx) (hax : ax_consist AX Γ) : ∃ Γ', max_ax_consist AX Γ' ∧ Γ ⊆ Γ' :=
 begin
 let S := { Γ'' | Γ'' ⊇ Γ ∧ ax_consist AX Γ''},
@@ -204,3 +257,14 @@ end
 -- by induction on L.
 -- S := collection of max cons sets
 -- m := Γ'
+
+
+
+-- Corollary 8
+lemma max_ax_exists (AX : ctx) : ∃ Γ : ctx, max_ax_consist AX Γ :=
+begin
+have hax : ax_consist AX ∅, 
+{rw ax_consist, intros L h1, rw fin_ax_consist, by_contradiction h2, sorry},
+have h1 : ∃ Γ, max_ax_consist AX Γ ∧ ∅ ⊆ Γ, from lindenbaum AX ∅ hax, 
+cases h1 with Γ h1, cases h1 with h1 h2, existsi (Γ : ctx), apply h1
+end
