src/del/semantics/complexitylemmas.lean
@@ -55,10 +55,9 @@ have h2 := add_comm _ _,
 exact (eq.subst h2 (lt_of_le_of_lt (le_max_right (complexity φ) (complexity ψ)) h1))
 end
 
-lemma tr3 : ∀ φ : formPA agents, 1 + max (complexity φ) 1 < 4 + complexity φ :=
+lemma tr3 : ∀ φ : formPA agents, 1 + max (complexity φ) 1 < complexity φ + 4 :=
 begin
 intro φ,
-rw add_comm 4,
 have h1 : complexity φ < complexity φ + 1, from lt_add_one _,
 have h2 : 0 < 2 ↔ 2 ≠ 0, from zero_lt_iff_ne_zero,
 cases h2, 
@@ -151,11 +150,10 @@ have h5 : 1 + (complexity φ + 4) * complexity χ ≤ 1 + (complexity φ + 4) * 
 exact (lt_of_le_of_lt h5 tr5helper)
 end
 
-lemma tr5 : ∀ φ ψ χ : formPA agents, 1 + max ((4 + complexity φ) * complexity ψ) 
-  ((4 + complexity φ) * complexity χ) < (4 + complexity φ) * (1 + max (complexity ψ) (complexity χ)) :=
+lemma tr5 : ∀ φ ψ χ : formPA agents, 1 + max ((complexity φ + 4) * complexity ψ) 
+  ((complexity φ + 4) * complexity χ) < (complexity φ + 4) * (1 + max (complexity ψ) (complexity χ)) :=
 begin
 intros φ ψ χ,
-rw add_comm 4,
 cases max_choice (complexity ψ) (complexity χ),
 cases max_choice ((complexity φ + 4) * complexity ψ) ((complexity φ + 4) * complexity χ),
 exact (eq.substr h_1 (eq.substr h (tr5helper))),
@@ -178,14 +176,6 @@ have h6 : 1 + complexity φ < (complexity φ + 4) * (complexity ψ + 1), linarit
 have h7 : 1 + 1 + (complexity φ + 4) * complexity ψ = 1 + (1 + (complexity φ + 4) * complexity ψ), linarith,
 have h8 : 1 + complexity ψ = complexity ψ + 1, linarith,
 exact (maxhelper h6 (eq.subst h8 (eq.subst h7 tr4helper2)))
-end
-
-lemma tr6' : ∀ φ ψ : formPA agents, 1 + max (complexity φ) (1 + (4 + complexity φ) 
-  * complexity ψ) < (4 + complexity φ) * (1 + complexity ψ) :=
-begin
-  intros φ ψ,
-  rw add_comm 4, rw add_comm 1 (complexity ψ),
-  apply tr6
 end
 
 lemma tr7helper1 {φ ψ : formPA agents} : (complexity φ + 4) * (complexity ψ + 4) 
@@ -254,22 +244,6 @@ have h3 : (1 + 4 + max (complexity φ) ((complexity φ + 4) * complexity ψ))
 exact (eq.subst h1 (mul_lt_mul_of_pos_right (eq.subst h3 (maxhelper tr7helper3 tr7helper6)) comp_gt_zero))
 end
 
-lemma tr7' : ∀ φ ψ χ : formPA agents, (4 + (1 + max (complexity φ) ((4 + complexity φ) 
-  * complexity ψ))) * complexity χ < (4 + complexity φ) * ((4 + complexity ψ) * complexity χ) :=
-begin
-  intros φ ψ χ,
-  rw [add_left_comm 4, add_comm 4 (complexity φ), add_comm 4 (complexity ψ)],
-  apply tr7
-end
-
-/-
-
-  (1 + (4 + max (complexity φ) ((complexity φ + 4) * complexity ψ))) * complexity χ <
-    (complexity φ + 4) * ((complexity ψ + 4) * complexity χ)
-⊢ (4 + (1 + max (complexity φ) ((4 + complexity φ) * complexity ψ))) * complexity χ <
-    (4 + complexity φ) * ((4 + complexity ψ) * complexity χ)
-
--/
 
 -------------- Helper lemmas for equiv_translation_aux --------------
 
