src/del/semantics/translationfunction.lean
@@ -10,9 +10,8 @@ variables {agents : Type}
   | (K a φ)          := K a (translate φ)
   | (U φ formPA.bot) := have _, from tr3 φ,     translate (φ ⊃ ⊥)
   | (U φ (p n))      := have _, from tr3 φ,     translate (φ ⊃ (p n))
-  | (U φ (~ψ))       := have _, from tr4 φ ψ,   translate (φ ⊃ ~ (U φ ψ))
   | (U φ (ψ & χ))    := have _, from tr5 φ ψ χ, translate ((U φ ψ) & (U φ χ))
   | (U φ (ψ ⊃ χ))    := have _, from tr5 φ ψ χ, translate ((U φ ψ) ⊃ (U φ χ))
-  | (U φ (K a ψ))    := have _, from tr6' φ ψ,   translate (φ ⊃ (K a (U φ ψ)))
-  | (U φ (U ψ χ))    := have _, from tr7' φ ψ χ, translate (U (φ & (U φ ψ)) χ)
+  | (U φ (K a ψ))    := have _, from tr6 φ ψ,   translate (φ ⊃ (K a (U φ ψ)))
+  | (U φ (U ψ χ))    := have _, from tr7 φ ψ χ, translate (U (φ & (U φ ψ)) χ)
   using_well_founded { rel_tac := λ _ _, `[exact ⟨_, measure_wf complexity⟩] }
